arm/ValueAOp.v
@@ -21,30 +21,36 @@ Require Import Op.
 Require Import ValueDomain.
 Require Import RTL.
 
-(** Value analysis for IA32 operators *)
+(** Value analysis for ARM operators *)
+
+Definition eval_static_shift (s: shift) (v: aval): aval :=
+  match s with
+  | Slsl x => shl v (I x)
+  | Slsr x => shru v (I x)
+  | Sasr x => shr v (I x)
+  | Sror x => ror v (I x)
+  end.
 
 Definition eval_static_condition (cond: condition) (vl: list aval): abool :=
   match cond, vl with
   | Ccomp c, v1 :: v2 :: nil => cmp_bool c v1 v2
   | Ccompu c, v1 :: v2 :: nil => cmpu_bool c v1 v2
+  | Ccompshift c s, v1 :: v2 :: nil => cmp_bool c v1 (eval_static_shift s v2)
+  | Ccompushift c s, v1 :: v2 :: nil => cmpu_bool c v1 (eval_static_shift s v2)
   | Ccompimm c n, v1 :: nil => cmp_bool c v1 (I n)
   | Ccompuimm c n, v1 :: nil => cmpu_bool c v1 (I n)
   | Ccompf c, v1 :: v2 :: nil => cmpf_bool c v1 v2
   | Cnotcompf c, v1 :: v2 :: nil => cnot (cmpf_bool c v1 v2)
-  | Cmaskzero n, v1 :: nil => maskzero v1 n
-  | Cmasknotzero n, v1 :: nil => cnot (maskzero v1 n)
+  | Ccompfzero c, v1 :: nil => cmpf_bool c v1 (F Float.zero)
+  | Cnotcompfzero c, v1 :: nil => cnot (cmpf_bool c v1 (F Float.zero))
   | _, _ => Bnone
   end.
 
 Definition eval_static_addressing (addr: addressing) (vl: list aval): aval :=
   match addr, vl with
   | Aindexed n, v1::nil => add v1 (I n)
-  | Aindexed2 n, v1::v2::nil => add (add v1 v2) (I n)
-  | Ascaled sc ofs, v1::nil => add (mul v1 (I sc)) (I ofs)
-  | Aindexed2scaled sc ofs, v1::v2::nil => add v1 (add (mul v2 (I sc)) (I ofs))
-  | Aglobal s ofs, nil => Ptr (Gl s ofs)
-  | Abased s ofs, v1::nil => add (Ptr (Gl s ofs)) v1
-  | Abasedscaled sc s ofs, v1::nil => add (Ptr (Gl s ofs)) (mul v1 (I sc))
+  | Aindexed2, v1::v2::nil => add v1 v2
+  | Aindexed2shift s, v1::v2::nil => add v1 (eval_static_shift s v2)
   | Ainstack ofs, nil => Ptr(Stk ofs)
   | _, _ => Vbot
   end.
@@ -54,37 +60,41 @@ Definition eval_static_operation (op: operation) (vl: list aval): aval :=
   | Omove, v1::nil => v1
   | Ointconst n, nil => I n
   | Ofloatconst n, nil => if propagate_float_constants tt then F n else ftop
-  | Oindirectsymbol id, nil => Ptr (Gl id Int.zero)
+  | Oaddrsymbol id ofs, nil => Ptr (Gl id ofs)
+  | Oaddrstack ofs, nil => Ptr (Stk ofs)
   | Ocast8signed, v1 :: nil => sign_ext 8 v1
-  | Ocast8unsigned, v1 :: nil => zero_ext 8 v1
   | Ocast16signed, v1 :: nil => sign_ext 16 v1
-  | Ocast16unsigned, v1 :: nil => zero_ext 16 v1
-  | Oneg, v1::nil => neg v1
+  | Oadd, v1::v2::nil => add v1 v2
+  | Oaddshift s, v1::v2::nil => add v1 (eval_static_shift s v2)
+  | Oaddimm n, v1::nil => add v1 (I n)
   | Osub, v1::v2::nil => sub v1 v2
+  | Osubshift s, v1::v2::nil => sub v1 (eval_static_shift s v2)
+  | Orsubshift s, v1::v2::nil => sub (eval_static_shift s v2) v1
+  | Orsubimm n, v1::nil => sub (I n) v1
   | Omul, v1::v2::nil => mul v1 v2
-  | Omulimm n, v1::nil => mul v1 (I n)
+  | Omla, v1::v2::v3::nil => add (mul v1 v2) v3
   | Omulhs, v1::v2::nil => mulhs v1 v2
   | Omulhu, v1::v2::nil => mulhu v1 v2
   | Odiv, v1::v2::nil => divs v1 v2
   | Odivu, v1::v2::nil => divu v1 v2
-  | Omod, v1::v2::nil => mods v1 v2
-  | Omodu, v1::v2::nil => modu v1 v2
   | Oand, v1::v2::nil => and v1 v2
+  | Oandshift s, v1::v2::nil => and v1 (eval_static_shift s v2)
   | Oandimm n, v1::nil => and v1 (I n)
   | Oor, v1::v2::nil => or v1 v2
+  | Oorshift s, v1::v2::nil => or v1 (eval_static_shift s v2)
   | Oorimm n, v1::nil => or v1 (I n)
   | Oxor, v1::v2::nil => xor v1 v2
+  | Oxorshift s, v1::v2::nil => xor v1 (eval_static_shift s v2)
   | Oxorimm n, v1::nil => xor v1 (I n)
+  | Obic, v1::v2::nil => and v1 (notint v2)
+  | Obicshift s, v1::v2::nil => and v1 (notint (eval_static_shift s v2))
+  | Onot, v1::nil => notint v1
+  | Onotshift s, v1::nil => notint (eval_static_shift s v1)
   | Oshl, v1::v2::nil => shl v1 v2
-  | Oshlimm n, v1::nil => shl v1 (I n)
   | Oshr, v1::v2::nil => shr v1 v2
-  | Oshrimm n, v1::nil => shr v1 (I n)
-  | Oshrximm n, v1::nil => shrx v1 (I n)
   | Oshru, v1::v2::nil => shru v1 v2
-  | Oshruimm n, v1::nil => shru v1 (I n)
-  | Ororimm n, v1::nil => ror v1 (I n)
-  | Oshldimm n, v1::v2::nil => or (shl v1 (I n)) (shru v2 (I (Int.sub Int.iwordsize n)))
-  | Olea addr, _ => eval_static_addressing addr vl
+  | Oshift s, v1::nil => eval_static_shift s v1
+  | Oshrximm n, v1::nil => shrx v1 (I n)
   | Onegf, v1::nil => negf v1
   | Oabsf, v1::nil => absf v1
   | Oaddf, v1::v2::nil => addf v1 v2
@@ -93,7 +103,9 @@ Definition eval_static_operation (op: operation) (vl: list aval): aval :=
   | Odivf, v1::v2::nil => divf v1 v2
   | Osingleoffloat, v1::nil => singleoffloat v1
   | Ointoffloat, v1::nil => intoffloat v1
+  | Ointuoffloat, v1::nil => intuoffloat v1
   | Ofloatofint, v1::nil => floatofint v1
+  | Ofloatofintu, v1::nil => floatofintu v1
   | Omakelong, v1::v2::nil => longofwords v1 v2
   | Olowlong, v1::nil => loword v1
   | Ohighlong, v1::nil => hiword v1
@@ -108,6 +120,16 @@ Variable ge: genv.
 Hypothesis GENV: genv_match bc ge.
 Variable sp: block.
 Hypothesis STACK: bc sp = BCstack.
+
+Lemma eval_static_shift_sound:
+  forall s v a,
+  vmatch bc v a ->
+  vmatch bc (eval_shift s v) (eval_static_shift s a).
+Proof.
+  intros. unfold eval_shift, eval_static_shift. destruct s; eauto with va.
+Qed.
+
+Hint Resolve eval_static_shift_sound: va.
 
 Theorem eval_static_condition_sound:
   forall cond vargs m aargs,
@@ -162,7 +184,8 @@ Proof.
   unfold eval_operation, eval_static_operation; intros;
   destruct op; InvHyps; eauto with va.
   destruct (propagate_float_constants tt); constructor.
-  eapply eval_static_addressing_sound; eauto.
+  rewrite Int.add_zero_l; eauto with va.
+  fold (Val.sub (Vint i) a1). auto with va.
   apply of_optbool_sound. eapply eval_static_condition_sound; eauto. 
 Qed.
 
