arm/CombineOp.v
@@ -17,13 +17,7 @@ Require Import Coqlib.
 Require Import AST.
 Require Import Integers.
 Require Import Op.
-Require SelectOp.
-
-Definition valnum := positive.
-
-Inductive rhs : Type :=
-  | Op: operation -> list valnum -> rhs
-  | Load: memory_chunk -> addressing -> list valnum -> rhs.
+Require Import CSEdomain.
 
 Section COMBINE.
 
@@ -104,7 +98,9 @@ Function combine_op (op: operation) (args: list valnum) : option(operation * lis
       end
   | Oandimm n, x :: nil =>
       match get x with
-      | Some(Op (Oandimm m) ys) => Some(Oandimm (Int.and m n), ys)
+      | Some(Op (Oandimm m) ys) => 
+          Some(let p := Int.and m n in
+               if Int.eq p m then (Omove, x :: nil) else (Oandimm p, ys))
       | _ => None
       end
   | Oorimm n, x :: nil =>
