arm/NeedOp.v
@@ -1,0 +1,204 @@
+(* *********************************************************************)
+(*                                                                     *)
+(*              The Compcert verified compiler                         *)
+(*                                                                     *)
+(*          Xavier Leroy, INRIA Paris-Rocquencourt                     *)
+(*                                                                     *)
+(*  Copyright Institut National de Recherche en Informatique et en     *)
+(*  Automatique.  All rights reserved.  This file is distributed       *)
+(*  under the terms of the INRIA Non-Commercial License Agreement.     *)
+(*                                                                     *)
+(* *********************************************************************)
+
+Require Import Coqlib.
+Require Import AST.
+Require Import Integers.
+Require Import Floats.
+Require Import Values.
+Require Import Memory.
+Require Import Globalenvs.
+Require Import Op.
+Require Import NeedDomain.
+Require Import RTL.
+
+(** Neededness analysis for ARM operators *)
+
+Definition needs_of_condition (cond: condition): list nval := nil.
+
+Definition needs_of_shift (s: shift) (nv: nval): nval :=
+  match s with
+  | Slsl x => shlimm nv x
+  | Slsr x => shruimm nv x
+  | Sasr x => shrimm nv x
+  | Sror x => ror nv x
+  end.
+
+Definition op1 (nv: nval) := nv :: nil.
+Definition op2 (nv: nval) := nv :: nv :: nil.
+Definition op2shift (s: shift) (nv: nval) := nv :: needs_of_shift s nv :: nil.
+
+Definition needs_of_operation (op: operation) (nv: nval): list nval :=
+  match op with
+  | Omove => nv::nil
+  | Ointconst n => nil
+  | Ofloatconst n => nil
+  | Oaddrsymbol id ofs => nil
+  | Oaddrstack ofs => nil
+  | Ocast8signed => op1 (sign_ext 8 nv)
+  | Ocast16signed => op1 (sign_ext 16 nv)
+  | Oadd => op2 (modarith nv)
+  | Oaddshift s => op2shift s (modarith nv)
+  | Oaddimm _ => op1 (modarith nv)
+  | Osub => op2 (default nv)
+  | Osubshift s => op2shift s (default nv)
+  | Orsubshift s => op2shift s (default nv)
+  | Orsubimm _ => op1 (default nv)
+  | Omul => op2 (modarith nv)
+  | Omla => let n := modarith nv in let n2 := modarith n in n2::n2::n::nil
+  | Omulhu | Omulhs | Odiv | Odivu => let n := default nv in n::n::nil
+  | Oand => op2 (bitwise nv)
+  | Oandshift s => op2shift s (bitwise nv)
+  | Oandimm n => op1 (andimm nv n)
+  | Oor => op2 (bitwise nv)
+  | Oorshift s => op2shift s (bitwise nv)
+  | Oorimm n => op1 (orimm nv n)
+  | Oxor => op2 (bitwise nv)
+  | Oxorshift s => op2shift s (bitwise nv)
+  | Oxorimm n => op1 (bitwise nv)
+  | Obic => let n := bitwise nv in n::bitwise n::nil
+  | Obicshift s => let n := bitwise nv in n::needs_of_shift s (bitwise n)::nil
+  | Onot => op1 (bitwise nv)
+  | Onotshift s => op1 (needs_of_shift s (bitwise nv))
+  | Oshl | Oshr | Oshru => op2 (default nv)
+  | Oshift s => op1 (needs_of_shift s nv)
+  | Oshrximm _ => op1 (default nv)
+  | Onegf | Oabsf => op1 (default nv)
+  | Oaddf | Osubf | Omulf | Odivf => op2 (default nv)
+  | Osingleoffloat => op1 (singleoffloat nv)
+  | Ointoffloat | Ointuoffloat | Ofloatofint | Ofloatofintu => op1 (default nv)
+  | Omakelong => op2 (default nv)
+  | Olowlong | Ohighlong => op1 (default nv)
+  | Ocmp c => needs_of_condition c
+  end.
+
+Definition operation_is_redundant (op: operation) (nv: nval): bool :=
+  match op with
+  | Ocast8signed => sign_ext_redundant 8 nv
+  | Ocast16signed => sign_ext_redundant 16 nv
+  | Oandimm n => andimm_redundant nv n
+  | Oorimm n => orimm_redundant nv n
+  | Osingleoffloat => singleoffloat_redundant nv
+  | _ => false
+  end.
+
+Ltac InvAgree :=
+  match goal with
+  | [H: vagree_list nil _ _ |- _ ] => inv H; InvAgree
+  | [H: vagree_list (_::_) _ _ |- _ ] => inv H; InvAgree
+  | _ => idtac
+  end.
+
+Ltac TrivialExists :=
+  match goal with
+  | [ |- exists v, Some ?x = Some v /\ _ ] => exists x; split; auto
+  | _ => idtac
+  end.
+
+Section SOUNDNESS.
+
+Variable ge: genv.
+Variable sp: block.
+Variables m m': mem.
+Hypothesis PERM: forall b ofs k p, Mem.perm m b ofs k p -> Mem.perm m' b ofs k p.
+
+Lemma needs_of_condition_sound:
+  forall cond args b args',
+  eval_condition cond args m = Some b ->
+  vagree_list args args' (needs_of_condition cond) ->
+  eval_condition cond args' m' = Some b.
+Proof.
+  intros. unfold needs_of_condition in H0. 
+  eapply default_needs_of_condition_sound; eauto.
+Qed.
+
+Lemma needs_of_shift_sound:
+  forall v v' s nv,
+  vagree v v' (needs_of_shift s nv) ->
+  vagree (eval_shift s v) (eval_shift s v') nv.
+Proof.
+  intros. destruct s; simpl in *. 
+  apply shlimm_sound; auto.
+  apply shruimm_sound; auto.
+  apply shrimm_sound; auto. 
+  apply ror_sound; auto.
+Qed.
+
+Lemma val_sub_lessdef:
+  forall v1 v1' v2 v2',
+  Val.lessdef v1 v1' -> Val.lessdef v2 v2' -> Val.lessdef (Val.sub v1 v2) (Val.sub v1' v2').
+Proof.
+  intros. inv H. inv H0. auto. destruct v1'; simpl; auto. simpl; auto.
+Qed.
+
+Lemma needs_of_operation_sound:
+  forall op args v nv args',
+  eval_operation ge (Vptr sp Int.zero) op args m = Some v ->
+  vagree_list args args' (needs_of_operation op nv) ->
+  nv <> Nothing ->
+  exists v',
+     eval_operation ge (Vptr sp Int.zero) op args' m' = Some v'
+  /\ vagree v v' nv.
+Proof.
+  unfold needs_of_operation; intros; destruct op; try (eapply default_needs_of_operation_sound; eauto; fail);
+  simpl in *; FuncInv; InvAgree; TrivialExists.
+- apply sign_ext_sound; auto. compute; auto.
+- apply sign_ext_sound; auto. compute; auto.
+- apply add_sound; auto.
+- apply add_sound; auto. apply needs_of_shift_sound; auto. 
+- apply add_sound; auto with na.
+- replace (default nv) with All in *. 
+  apply vagree_lessdef. apply val_sub_lessdef; auto with na. 
+  apply lessdef_vagree. apply needs_of_shift_sound; auto with na.
+  destruct nv; simpl; congruence.
+- replace (default nv) with All in *. 
+  apply vagree_lessdef. apply val_sub_lessdef; auto with na. 
+  apply lessdef_vagree. apply needs_of_shift_sound; auto with na.
+  destruct nv; simpl; congruence.
+- apply mul_sound; auto. 
+- apply add_sound; auto. apply mul_sound; auto. 
+- apply and_sound; auto.
+- apply and_sound; auto. apply needs_of_shift_sound; auto. 
+- apply andimm_sound; auto.
+- apply or_sound; auto.
+- apply or_sound; auto. apply needs_of_shift_sound; auto. 
+- apply orimm_sound; auto.
+- apply xor_sound; auto.
+- apply xor_sound; auto. apply needs_of_shift_sound; auto. 
+- apply xor_sound; auto with na.
+- apply and_sound; auto. apply notint_sound; auto. 
+- apply and_sound; auto. apply notint_sound. apply needs_of_shift_sound; auto. 
+- apply notint_sound; auto. 
+- apply notint_sound. apply needs_of_shift_sound; auto.
+- apply needs_of_shift_sound; auto. 
+- apply singleoffloat_sound; auto. 
+Qed.
+
+Lemma operation_is_redundant_sound:
+  forall op nv arg1 args v arg1' args',
+  operation_is_redundant op nv = true ->
+  eval_operation ge (Vptr sp Int.zero) op (arg1 :: args) m = Some v ->
+  vagree_list (arg1 :: args) (arg1' :: args') (needs_of_operation op nv) ->
+  vagree v arg1' nv.
+Proof.
+  intros. destruct op; simpl in *; try discriminate; inv H1; FuncInv; subst.
+- apply sign_ext_redundant_sound; auto. omega.
+- apply sign_ext_redundant_sound; auto. omega.
+- apply andimm_redundant_sound; auto. 
+- apply orimm_redundant_sound; auto.
+- apply singleoffloat_redundant_sound; auto.
+Qed.
+
+End SOUNDNESS.
+
+
+
